eclib/JArray.ec
@@ -99,7 +99,7 @@ abstract theory MonoArray.
     k1 = k2 => t.[k1 <- x].[k2 <- x'] = t.[k2 <- x'].
   proof. move=> ->; apply set_set_eq. qed.
 
-  hint simplify (set_set_eq_s, set_out).
+  hint simplify set_out.
 
   lemma set_set_swap (t : t) (k k' : int) (x x' : elem):
     k <> k' => t.[k <- x].[k' <- x'] = t.[k' <- x'].[k <- x].
@@ -149,9 +149,9 @@ abstract theory MonoArray.
   lemma to_list_inj : injective to_list.
   proof. by apply/(can_inj _ _ to_listK). qed.
 
-  hint simplify (get_of_list, get_to_list)@0.
+  hint simplify (get_of_list, get_to_list, size_to_list)@0.
   hint simplify [reduce] to_listK@0.
-  hint simplify [reduce] to_listE@1.
+(*  hint simplify [reduce] to_listE@1. *)
 
   lemma init_of_list f : init f = of_list (map f (iota_ 0 size)).
   proof.
@@ -177,7 +177,7 @@ abstract theory MonoArray.
   lemma createL (a:elem) : create a = of_list (map (fun i => a) (iota_ 0 size)).
   proof. by rewrite /create init_of_list. qed.
 
-  hint simplify (createiE, createL).
+  hint simplify createiE @0.
 
   (* -------------------------------------------------------------------- *)
   op map (f: elem -> elem) (t:t) : t =
@@ -219,11 +219,14 @@ abstract theory MonoArray.
   proof.
     rewrite to_listE map2E map2_zip init_of_list /=;congr.
     apply (eq_from_nth dfl).
-    + by rewrite !size_map size_zip !size_map StdOrder.IntOrder.minrE. 
+    + rewrite !size_map size_zip !size_map StdOrder.IntOrder.minrE /=. 
+      smt (size_iota ge0_size).
     move=> i; rewrite size_map => hi.
     rewrite (nth_map 0) 1:// (nth_map (dfl,dfl)).
-    + by rewrite size_zip StdOrder.IntOrder.minrE /= !size_map.
-    by rewrite /= nth_zip ?size_map // !(nth_map 0).
+    + rewrite size_zip StdOrder.IntOrder.minrE /= !size_map.
+      smt (size_iota ge0_size).
+    rewrite /= nth_zip ?size_map //=; 1: smt (size_iota ge0_size).
+    rewrite !(nth_map 0) // !nth_iota //; smt (ge0_size size_iota).
   qed.
 
   hint simplify (map2iE, map2_of_list)@0.
@@ -231,11 +234,11 @@ abstract theory MonoArray.
 
   (* -------------------------------------------------------------------- *)
   op all_eq (t1 t2: t) =
-    all (fun x => t1.[x] = t2.[x]) (iota_ 0 size).
+    all (fun x => t1.[x] = t2.[x]) (iotared 0 size).
 
   lemma all_eq_eq (t1 t2: t) : all_eq t1 t2 => t1 = t2.
   proof.
-    by move=> /allP h; apply ext_eq => x /mem_range; apply h.
+    by move=> /allP h; apply ext_eq => x /mem_range hx; apply h; rewrite iotaredE.
   qed.
 
   lemma all_eqP (t1 t2: t) : all_eq t1 t2 <=> t1 = t2.
@@ -397,13 +400,13 @@ abstract theory PolyArray.
 
   (* -------------------------------------------------------------------- *)
   op all_eq (t1 t2: 'a t) =
-    all (fun x => t1.[x] = t2.[x]) (iota_ 0 size).
+    all (fun x => t1.[x] = t2.[x]) (iotared 0 size).
 
   lemma ext_eq_all (t1 t2: 'a t) :
     all_eq t1 t2 <=> t1 = t2.
   proof.
     split.
-    + by move=> /allP h; apply ext_eq => x /mem_range; apply h.
+    + by move=> /allP h; apply ext_eq => x /mem_range hx; apply h; rewrite iotaredE.
     by move=> ->;apply /allP.
   qed.
 
